Refactored equivocator states to always have projection 0

VLSM/Equivocators.v
@@ -67,7 +67,7 @@ Inductive MachineDescriptor : Type
 
 
 Definition equivocator_type : VLSM_type message :=
-  {| state := {n : nat & Fin.t n -> vstate X};
+  {| state := {n : nat & Fin.t (S n) -> vstate X};
      label := vlabel X * MachineDescriptor
   |}.
 
@@ -77,7 +77,7 @@ Definition mk_singleton_state
   (s : vstate X)
   : equivocator_state
   :=
-  existT _ 1 (fun _ => s).
+  existT _ 0 (fun _ => s).
 
 Definition equivocator_label : Type := @label message equivocator_type.
 
@@ -93,7 +93,7 @@ Definition equivocator_state_project
   : option (vstate X)
   :=
   let (n, s) := bs in
-  match (le_lt_dec n i) with
+  match (le_lt_dec (S n) i) with
   | right lt_in => Some (s (of_nat_lt lt_in))
   | _ =>  None
   end.
@@ -101,7 +101,7 @@ Definition equivocator_state_project
 Definition equivocator_state_update
   (bs : equivocator_state)
   (n := projT1 bs)
-  (i : Fin.t n)
+  (i : Fin.t (S n))
   (si : vstate X)
   : equivocator_state
   :=
@@ -117,31 +117,30 @@ Program Definition equivocator_state_extend
   existT _ (S n)
     (fun j =>
       let (nj, Hnj) := to_nat j in
-      if (nat_eq_dec nj n) then s else is (@of_nat_lt nj n _)
+      if (nat_eq_dec nj (S n)) then s else is (@of_nat_lt nj (S n) _)
     ).
 Next Obligation.
   lia.
 Defined.
 
+Lemma Hzero (s : equivocator_state) : 0 < S (projT1 s).
+Proof. lia. Qed.
+
 Definition equivocator_initial_state_prop
   (bs : equivocator_state)
   : Prop
-  := projT1 bs = 0.
+  := projT1 bs = 0 /\ vinitial_state_prop X (projT2 bs (of_nat_lt (Hzero bs))).
 
 Definition equivocator_initial_state
   := sig equivocator_initial_state_prop.
 
-Definition empty_fn
-  (i : Fin.t 0)
-  : vstate X.
-Proof.
-  dependent destruction i.
-Defined.
-
 Definition equivocator_s0 : equivocator_initial_state.
 Proof.
-  exists (existT _ 0 empty_fn).
-  unfold equivocator_initial_state_prop. reflexivity.
+  exists (mk_singleton_state (proj1_sig (vs0 X))).
+  unfold mk_singleton_state.
+  unfold equivocator_initial_state_prop.
+  split; try reflexivity.
+  simpl. destruct (vs0 X). assumption.
 Defined.
 
 Definition equivocator_l0 : equivocator_label :=
@@ -171,7 +170,7 @@ Definition equivocator_transition
     let (sn', om') := vtransition X l (sn, om) in
     (equivocator_state_extend bs sn', om')
   | Existing i is_equiv =>
-    match (le_lt_dec n i) with
+    match (le_lt_dec (S n) i) with
     | right lt_in =>
       let ni := of_nat_lt lt_in in
       let si := s ni in
@@ -198,7 +197,7 @@ Definition equivocator_valid
     vinitial_state_prop X sn
     /\ vvalid X l (sn, om)
   | Existing i is_equiv =>
-    exists (Hi : i < n), vvalid X l (s (of_nat_lt Hi), om)
+    exists (Hi : i < S n), vvalid X l (s (of_nat_lt Hi), om)
   end.
 
 Definition equivocator_vlsm_machine
@@ -216,33 +215,6 @@ Definition equivocator_vlsm
 Instance option_bool_eq : EqDec (option bool)
   := option_eq_dec Bool.bool_dec.
 
-Lemma equivocator_initial_state_empty
-  (s : vstate equivocator_vlsm)
-  (Hs : vinitial_state_prop equivocator_vlsm s)
-  (i : Fin.t (projT1 s))
-  : False.
-Proof.
-  unfold vinitial_state_prop in Hs. simpl in Hs.
-  unfold equivocator_initial_state_prop in Hs.
-  destruct s. simpl in *.
-  subst. inversion i.
-Qed.
-
-Lemma equivocator_initial_state_unique
-  (s : vstate equivocator_vlsm)
-  (Hs : vinitial_state_prop equivocator_vlsm s)
-  : s = proj1_sig (vs0 equivocator_vlsm).
-Proof.
-  destruct s as [ns bs]. 
-  unfold vs0. simpl.
-  unfold vinitial_state_prop in Hs. simpl in Hs.
-  unfold equivocator_initial_state_prop in Hs. simpl in Hs.
-  subst.
-  f_equal.
-  apply functional_extensionality.
-  intro i. inversion i.
-Qed.
-
 Definition equivocator_vlsm_transition_item_project
   (item : vtransition_item equivocator_vlsm)
   (descriptor : MachineDescriptor)
@@ -253,13 +225,13 @@ Definition equivocator_vlsm_transition_item_project
   | Existing j _ =>
     match item with {| l := (lx, descriptor); input := im; output := om; destination := s |} =>
       let (n, bs) := s in
-      match (le_lt_dec n j) with
+      match (le_lt_dec (S n) j) with
       | right lt_jn =>
         let nj := of_nat_lt lt_jn in
         let item' := {| l := lx; input := im; output := om; destination := bs nj|} in
         match descriptor with
         | NewMachine s =>
-          if nat_eq_dec (S j) n then (* this is the first state *)
+          if nat_eq_dec (S j) (S n) then (* this is the first state *)
             Some ( Some item', descriptor)
           else Some (None, Existing j false)
         | Existing i is_equiv =>
@@ -269,7 +241,7 @@ Definition equivocator_vlsm_transition_item_project
               Some ( Some item', descriptor)
             else Some (None, Existing j false)
           | true => (* forking, transition happens on forked copy *)
-            if nat_eq_dec (S j) n then
+            if nat_eq_dec (S j) (S n) then
               Some (Some item', descriptor)
             else Some (None, Existing j false)
           end
@@ -291,25 +263,29 @@ Lemma equivocator_vlsm_transition_item_project_some_inj
   (HitemX' : equivocator_vlsm_transition_item_project item idescriptor' = Some (Some itemX', odescriptor'))
   : i = i' /\ itemX = itemX' /\ odescriptor = odescriptor'.
 Proof.
-  simpl in *.
+  unfold equivocator_vlsm_transition_item_project in *.
+  unfold idescriptor in *. clear idescriptor.
+  unfold idescriptor' in *. clear idescriptor'.
   destruct item.
   destruct l as (ls, descriptor).
   destruct destination as (ndest, bdest).
-  destruct (le_lt_dec ndest i); try discriminate HitemX.
-  destruct (le_lt_dec ndest i'); try discriminate HitemX'.
+  destruct (le_lt_dec (S ndest) i); try discriminate HitemX.
+  destruct (le_lt_dec (S ndest) i'); try discriminate HitemX'.
   destruct descriptor as [sn | j fj].
-  - destruct (nat_eq_dec (S i) ndest); try discriminate HitemX.
+  - destruct (nat_eq_dec (S i) (S ndest)); try discriminate HitemX.
     inversion HitemX. subst. clear HitemX.
-    destruct (nat_eq_dec (S i') (S i)); try discriminate HitemX'.
-    inversion e. subst. inversion HitemX'. subst. clear HitemX'.
+    inversion e. subst i. clear e.
+    destruct (nat_eq_dec (S i') (S ndest)); try discriminate HitemX'.
+    inversion e. subst i'. inversion HitemX'. subst. clear HitemX'.
     replace (of_nat_lt l0) with (of_nat_lt l) by apply of_nat_ext.
     repeat split; reflexivity.
   - destruct fj as [|] eqn:Hfj.
-    + destruct (nat_eq_dec (S i) ndest); try discriminate HitemX.
+    + destruct (nat_eq_dec (S i) (S ndest)); try discriminate HitemX.
       inversion HitemX; subst. clear HitemX.
-      destruct (nat_eq_dec (S i') (S i)); try discriminate HitemX'.
+      inversion e. subst i. clear e.
+      destruct (nat_eq_dec (S i') (S ndest)); try discriminate HitemX'.
       inversion HitemX'; subst. clear HitemX'.
-      inversion e; subst; clear e.
+      inversion e; subst i'; clear e.
       replace (of_nat_lt l0) with (of_nat_lt l) by apply of_nat_ext.
       repeat split; reflexivity.
     + destruct (nat_eq_dec j i); try discriminate HitemX.
@@ -327,17 +303,17 @@ Lemma equivocator_transition_item_project_inv_none
     (i : nat)
     (is_equiv : bool)
     (Hdescriptor : descriptor = Existing i is_equiv),
-    projT1 (destination item) <= i.
+    projT1 (destination item) < i.
 Proof.
+  unfold equivocator_vlsm_transition_item_project in Hitem.
   destruct item.
   destruct descriptor as [s|i is_equiv]; try discriminate Hitem.
   exists i. exists is_equiv. exists eq_refl.
-  simpl in  *.
   destruct destination as (n, bs).
-  destruct (le_lt_dec n i); try assumption.
+  destruct (le_lt_dec (S n) i); try assumption.
   destruct l as (ls, [is | ix [|]]).
-  - destruct (nat_eq_dec (S i) n); discriminate Hitem.
-  - destruct (nat_eq_dec (S i) n); discriminate Hitem.
+  - destruct (nat_eq_dec (S i) (S n)); discriminate Hitem.
+  - destruct (nat_eq_dec (S i) (S n)); discriminate Hitem.
   - destruct (nat_eq_dec ix i); discriminate Hitem.
 Qed.
 
@@ -352,16 +328,17 @@ Lemma equivocator_transition_item_project_inv_messages
     (Hdescriptor : idescriptor = Existing i is_equiv),
     input item = input itemX /\ output item = output itemX.
 Proof.
+  unfold equivocator_vlsm_transition_item_project in Hitem.
   destruct idescriptor as [s|j fj]; try discriminate Hitem.
   exists j. exists fj. exists eq_refl.
-  destruct item. simpl in *.
+  destruct item.
   destruct destination as (n, bs).
   destruct l as (lx, descriptorx).
-  destruct (le_lt_dec n j); try discriminate Hitem.
+  destruct (le_lt_dec (S n) j); try discriminate Hitem.
   destruct descriptorx as [s | i' [|]] eqn:Hl; simpl.
-  - destruct (nat_eq_dec (S j) n); try discriminate Hitem.
+  - destruct (nat_eq_dec (S j) (S n)); try discriminate Hitem.
     inversion Hitem. subst. clear Hitem. repeat split; reflexivity.
-  - destruct (nat_eq_dec (S j) n); try discriminate Hitem.
+  - destruct (nat_eq_dec (S j) (S n)); try discriminate Hitem.
     inversion Hitem. subst. repeat split; reflexivity.
   - destruct (nat_eq_dec i' j); try discriminate Hitem.
     inversion Hitem. subst. repeat split; reflexivity.
@@ -479,6 +456,12 @@ Proof.
     ; inversion Hprefix; subst; reflexivity.
 Qed.
 
+Local Tactic Notation "unfold_transition"  hyp(H) :=
+  ( unfold transition in H; unfold equivocator_vlsm in H
+  ; unfold mk_vlsm in H; unfold machine in H
+  ; unfold projT2 in H; unfold equivocator_vlsm_machine in H
+  ; unfold equivocator_transition in H).
+
 Lemma equivocator_state_project_protocol
   (bs : vstate equivocator_vlsm)
   (om : option message)
@@ -486,34 +469,37 @@ Lemma equivocator_state_project_protocol
   :
   option_protocol_message_prop X om /\
   let (n, bs) := bs in
-  forall (i : Fin.t n), protocol_state_prop X (bs i).
+  forall (i : Fin.t (S n)), protocol_state_prop X (bs i).
 Proof.
   remember (bs, om) as bsom.
   generalize dependent om. generalize dependent bs.
-  induction Hbs; intros; inversion Heqbsom; subst; clear Heqbsom; split.
+  induction Hbs; intros; split; try (apply pair_equal_spec in Heqbsom; destruct Heqbsom as [Heqbs Heqom]; subst).
   - exists (proj1_sig (vs0 X)). apply protocol_initial_state.
-  - destruct is as [is His]. unfold s; clear s.
-    destruct is as ([| [|n]], is); try inversion His. simpl in *.
-    intro i. inversion i.
+  - destruct is as [is His]. unfold s; clear s. simpl.
+    destruct His as [Hzero His].
+    destruct is as (n, is). simpl in Hzero. subst n. simpl in His.
+    intro i. dependent destruction i; try inversion i.
+    exists None. replace (is F1) with (proj1_sig (exist _ _ His)) by reflexivity.
+    apply protocol_initial_state.
   - unfold om; clear om.
     exists (proj1_sig (vs0 X)). apply (protocol_initial_message X).
   - unfold s; clear s. unfold s0. simpl.
-    intro i. inversion i.
+    intro i. exists None. apply protocol_initial_state. 
   - specialize (IHHbs1 s _om eq_refl).
     specialize (IHHbs2 _s om eq_refl).
     specialize (protocol_generated X) as Hgen.
     simpl in Hv.
-    destruct l as (l, descriptor). simpl in *.
+    destruct l as (l, descriptor). simpl in Hv.
     destruct descriptor as [sn| i is_equiv].
-    + destruct s as (n, bs'); simpl in *.
-      destruct IHHbs2 as [Hom _].
-      clear Hbs2 _s.
-      destruct Hom as [_s Hom].
+    + simpl in Heqbsom.
       destruct Hv as [Hsn Hv].
       assert (Hbsnt : protocol_prop X (sn, None)).
       { replace sn with (proj1_sig (exist _ sn Hsn)) by reflexivity.
         apply protocol_initial_state.
       }
+      destruct IHHbs2 as [Hom _].
+      clear Hbs2 _s.
+      destruct Hom as [_s Hom].
       specialize (Hgen l sn None Hbsnt _s om Hom Hv).
       replace
         (@transition message (@type message X) (@sign message X)
@@ -523,12 +509,13 @@ Proof.
         in Hgen
         by reflexivity.
       destruct (vtransition X l (sn, om)) as (si', om') eqn:Ht.
-      exists si'. inversion H0. subst om'. assumption.
-    + destruct Hv as [Hi Hv].
-      destruct (le_lt_dec (projT1 s) i). { lia. }
+      exists si'. inversion Heqbsom. subst om'. assumption.
+    + unfold_transition Heqbsom.
+      unfold snd in Heqbsom. destruct Hv as [Hi Hv].
+      destruct (le_lt_dec (S (projT1 s)) i). { lia. }
       replace (of_nat_lt l0) with (of_nat_lt Hi) in *; try apply of_nat_ext.
       clear l0.
-      destruct s as (n, bs'); simpl in *.
+      destruct s as (n, bs').
       destruct IHHbs1 as [_ IHHbs1].
       spec IHHbs1 (of_nat_lt Hi).
       destruct IHHbs1 as [_om' Hbs't].
@@ -544,25 +531,28 @@ Proof.
         with (vtransition X l (bs' (of_nat_lt Hi), om))
         in Hgen
         by reflexivity.
+      simpl in *.
       destruct (vtransition X l (bs' (of_nat_lt Hi), om)) as (si', om') eqn:Ht.
       exists si'.
-      destruct is_equiv as [|]; inversion H0; subst; clear H0; assumption.
+      destruct is_equiv as [|]; inversion Heqbsom; subst; assumption.
   - destruct bs as (n, bs).
     intro j.
     specialize (IHHbs1 s _om eq_refl).
     destruct IHHbs1 as [_ IHHbs1].
     specialize (IHHbs2 _s om eq_refl).
     specialize (protocol_generated X) as Hgen.
-    destruct l as (l, descriptor). simpl in H0.
+    unfold_transition Heqbsom.
+    destruct l as (l, descriptor). unfold snd in Heqbsom.
     destruct descriptor as [sn | i is_equiv].
     + destruct Hv as [Hsn Hv].
-      destruct s as (n0, bs0); simpl in *.
+      destruct s as (n0, bs0).
       destruct IHHbs2 as [(_som, Hom) _].
       assert (Hbsnt : protocol_prop X (sn, None)).
       { replace sn with (proj1_sig (exist _ sn Hsn)) by reflexivity.
         apply protocol_initial_state.
       }
       specialize (Hgen l sn None Hbsnt _som om Hom Hv).
+      simpl in *.
       replace
         (@transition message (@type message X) (@sign message X)
         (@machine message X) l
@@ -571,13 +561,13 @@ Proof.
         in Hgen
         by reflexivity.
       destruct (vtransition X l (sn, om)) as (si', om') eqn:Ht.
-      inversion H0. clear H0.
-      subst n om'. apply inj_pairT2 in H2. subst.
+      inversion Heqbsom. clear Heqbsom.
+      subst n om'. apply inj_pairT2 in H1. subst.
       * destruct (to_nat j) as (nj, Hnj).
-        try destruct (nat_eq_dec  nj n0); try (exists om0; assumption).
+        try destruct (nat_eq_dec nj (S n0)); try (exists om0; assumption).
         apply IHHbs1.
     + destruct Hv as [Hi Hv].
-      destruct (le_lt_dec (projT1 s) i). { lia. }
+      destruct (le_lt_dec (S (projT1 s)) i). { lia. }
       replace (of_nat_lt l0) with (of_nat_lt Hi) in *; try apply of_nat_ext.
       clear l0.
       destruct s as (n0, bs0); simpl in *.
@@ -593,10 +583,10 @@ Proof.
         in Hgen
         by reflexivity.
       destruct (vtransition X l (bs0 (of_nat_lt Hi), om)) as (si', om') eqn:Ht.
-      destruct is_equiv as [|]; inversion H0; clear H0
-      ; subst n om'; apply inj_pairT2 in H2; subst.
+      destruct is_equiv as [|]; inversion Heqbsom; clear Heqbsom
+      ; subst n om'; apply inj_pairT2 in H1; subst.
       * destruct (to_nat j) as (nj, Hnj).
-        try destruct (nat_eq_dec  nj n0); try (exists om0; assumption).
+        try destruct (nat_eq_dec  nj (S n0)); try (exists om0; assumption).
         apply IHHbs1.
       * destruct (Fin.eq_dec (of_nat_lt Hi) j); try apply IHHbs1.
         exists om0. assumption.
@@ -607,7 +597,7 @@ Lemma equivocator_state_project_protocol_state
   (Hbs : protocol_state_prop equivocator_vlsm bs)
   :
   let (n, bs) := bs in
-  forall (i : Fin.t n), protocol_state_prop X (bs i).
+  forall (i : Fin.t (S n)), protocol_state_prop X (bs i).
 Proof.
   destruct Hbs as [om Hbs].
   apply equivocator_state_project_protocol in Hbs.
@@ -641,7 +631,7 @@ Lemma equivocator_protocol_transition_item_project_inv2
     (i : nat)
     (fi : bool)
     (Hdi : di = Existing i fi)
-    (Hi : i < projT1 s)
+    (Hi : i < S (projT1 s))
     (sx := projT2 s (of_nat_lt Hi))
     (Hitem' : item' = {| l := fst l; input := iom; destination := sx; output := oom |}),
     match di' with
@@ -651,55 +641,59 @@ Lemma equivocator_protocol_transition_item_project_inv2
        vtransition X (fst l) (sn, iom) = (sx, oom)
     | Existing i' fi' =>
       exists
-       (Hi' : i' < projT1 s')
+       (Hi' : i' < S (projT1 s'))
        (s'x := projT2 s' (of_nat_lt Hi')),
        vvalid X (fst l) (s'x, iom) /\
        vtransition X (fst l) (s'x, iom) = (sx, oom)
   end.
 Proof.
   unfold vvalid in Hv. unfold vtransition in Ht.
-  simpl in Hv. simpl in Ht.
+  unfold_transition Ht.
+  simpl in Hv.
+  unfold equivocator_vlsm_transition_item_project in Hitem.
   destruct di as [sn| i fi]; try discriminate Hitem.
-  exists i. exists fi. exists eq_refl. simpl in Hitem.
+  exists i. exists fi. exists eq_refl. unfold item in Hitem.
   destruct l as (lx, descriptor).
   destruct s as (ns, bs).
-  destruct (le_lt_dec ns i); try discriminate Hitem.
-  exists l. simpl in Ht. simpl in Hv.
+  destruct (le_lt_dec (S ns) i); try discriminate Hitem.
+  exists l. unfold snd in Ht. unfold snd in Hv.
   destruct descriptor as [sn| j is_equiv].
-  - destruct (nat_eq_dec (S i) ns); try discriminate Hitem. subst ns.
+  - destruct (nat_eq_dec (S i) (S ns)); try discriminate Hitem.
+    inversion e. subst i. clear e.
     inversion Hitem. clear Hitem. exists eq_refl.
     destruct Hv as [Hsn Hv].
     repeat split; try assumption.
+    simpl in *.
     destruct (vtransition X lx (sn, iom)) as (sn', om') eqn:Htx.
     inversion Ht. subst. clear Ht. f_equal.
     destruct s' as (ns',bs'). simpl. simpl in H2.
     inversion H2; subst.
     apply inj_pairT2 in H2. subst.
     rewrite to_nat_of_nat.
-    destruct (nat_eq_dec i i); try elim n; try reflexivity. assumption.
+    destruct (nat_eq_dec (S ns') (S ns')); try elim n; reflexivity.
   - destruct Hv as [Hj Hv].
-    destruct (le_lt_dec (projT1 s') j). { lia. }
+    destruct (le_lt_dec (S (projT1 s')) j). { lia. }
     replace (of_nat_lt l0) with (of_nat_lt Hj) in *; try apply of_nat_ext. clear l0.
+    simpl in Ht.
     destruct (vtransition X lx (projT2 s' (of_nat_lt Hj), iom))
       as (si', om') eqn:Htx.
     destruct s' as (n', bs').
-    simpl in *.
     destruct is_equiv as [|].
-    + destruct (nat_eq_dec (S i) ns); try discriminate Hitem.
+    + destruct (nat_eq_dec (S i) (S ns)); try discriminate Hitem.
       inversion Hitem. subst di' item'. clear Hitem.
       exists eq_refl.
       exists Hj. split; try assumption.
-      inversion Ht. subst. clear Ht. inversion H0. subst i. clear H0.
-      apply inj_pairT2 in H1. subst.
-      rewrite to_nat_of_nat in *.
-      destruct (nat_eq_dec n' n'); try assumption.
+      inversion Ht. subst. clear Ht. inversion e. subst i. clear e.
+      apply inj_pairT2 in H1. subst. simpl.
+      rewrite to_nat_of_nat.
+      destruct (nat_eq_dec (S n') (S n')); try assumption.
       elim n. reflexivity.
     + destruct (nat_eq_dec j i); try discriminate Hitem. subst.
       inversion Hitem. subst di' item'. clear Hitem.
       exists eq_refl.
       exists Hj. split; try assumption.
       inversion Ht. subst. clear Ht.
-      apply inj_pairT2 in H1. subst.
+      apply inj_pairT2 in H1. subst. simpl.
       rewrite eq_dec_if_true; try apply of_nat_ext.
       assumption.
 Qed.
@@ -717,65 +711,68 @@ Lemma equivocator_protocol_transition_item_project_inv3
     | NewMachine sn => di' = di
     | Existing i fi =>
       exists
-        (Hi : i < projT1 s)
+        (Hi : i < S (projT1 s))
         (i' : nat)
         (fi' : bool)
         (Hdi' : di' = Existing i' fi')
-        (Hi' : i' < projT1 s'),
+        (Hi' : i' < S (projT1 s')),
         projT2 s' (of_nat_lt Hi') = projT2 s (of_nat_lt Hi)
     end.
 Proof.
   unfold vvalid in Hv. unfold vtransition in Ht.
   destruct l as (lx, d).
-  simpl in Hv. simpl in Ht.
+  simpl in Hv. unfold_transition Ht. unfold snd in Ht.
+  unfold equivocator_vlsm_transition_item_project in Hitem.
   destruct di as [si | i fi]; try (inversion Hitem; reflexivity).
-  simpl in Hv.
-  destruct d as [sd | id fd]; simpl in Hitem.
-  - destruct s as (ns, bs). destruct (le_lt_dec ns i); try discriminate Hitem.
-    destruct (nat_eq_dec (S i) ns); try discriminate Hitem.
+  simpl in Hv. unfold item in Hitem.
+  destruct s as (ns, bs).
+  destruct (le_lt_dec (S ns) i); try discriminate Hitem.
+  destruct d as [sd | id fd].
+  - destruct (nat_eq_dec (S i) (S ns)); try discriminate Hitem.
     simpl. exists l. inversion Hitem. subst. clear Hitem.
     exists i. exists false. exists eq_refl.
+    simpl in *.
     destruct (vtransition X lx (sd, iom)) as (sn', om').
     destruct s' as (ns', bs'). simpl in Ht.
     inversion Ht. subst.
     apply inj_pairT2 in H1.
     simpl.
-    assert (Hi' : i < ns') by lia.
+    assert (Hi' : i < S ns') by lia.
     exists Hi'.
     subst. rewrite to_nat_of_nat.
-    destruct (nat_eq_dec i ns'). { lia. }
+    destruct (nat_eq_dec i (S ns')). { lia. }
     f_equal. apply of_nat_ext.
   - destruct Hv as [Hj Hv].
-    destruct (le_lt_dec (projT1 s') id). { lia. }
-    replace (of_nat_lt l) with (of_nat_lt Hj) in *; try apply of_nat_ext. clear l.
-    destruct s as (n, bs).
+    destruct (le_lt_dec (S (projT1 s')) id). { lia. }
+    replace (of_nat_lt l0) with (of_nat_lt Hj) in *; try apply of_nat_ext. clear l0.
     destruct s' as (n', bs').
-    simpl in *.
-    destruct (le_lt_dec n i); try discriminate Hitem.
-    exists l.
-    destruct (vtransition X lx (bs' (of_nat_lt Hj), iom))
+    exists l. simpl in Ht.
+    destruct
+      (@vtransition message X lx
+      (@pair (@vstate message X) (option message)
+         (bs' (@of_nat_lt id (S n') Hj)) iom))
       as (si', om') eqn:Htx.
     destruct fd as [|].
-    + destruct (nat_eq_dec (S i) n); try discriminate Hitem.
+    + destruct (nat_eq_dec (S i) (S ns)); try discriminate Hitem.
       inversion Hitem. subst di'. clear Hitem.
       exists i. exists false. exists eq_refl.
       inversion Ht. subst. clear Ht.
-      assert (Hi : i < n') by lia.
+      assert (Hi : i < (S n')) by lia.
       exists Hi.
-      apply inj_pairT2 in H1. subst.
+      apply inj_pairT2 in H1. subst. simpl.
       rewrite to_nat_of_nat in *.
-      destruct (nat_eq_dec i n'). { lia. }
+      destruct (nat_eq_dec i (S n')). { lia. }
       f_equal.
       apply of_nat_ext.
     + destruct (nat_eq_dec id i); try discriminate Hitem.
       inversion Hitem. subst di'. clear Hitem.
       exists i. exists false. exists eq_refl.
       inversion Ht. subst. exists l.
-      apply inj_pairT2 in H1. subst.
+      apply inj_pairT2 in H1. subst. simpl.
       rewrite eq_dec_if_false; try reflexivity.
       intro contra. apply (f_equal to_nat) in contra.
       repeat rewrite to_nat_of_nat in contra.
-      inversion contra. elim n0. assumption.
+      inversion contra. elim n. assumption.
 Qed.
 
 Lemma equivocator_protocol_transition_item_project_inv4
@@ -786,43 +783,45 @@ Lemma equivocator_protocol_transition_item_project_inv4
   (Ht: vtransition equivocator_vlsm l (s', iom) = (s, oom))
   (i' : nat)
   (fi' : bool)
-  (Hi' : i' < projT1 s')
+  (Hi' : i' < S (projT1 s'))
   : exists
-    (Hi'' : i' < projT1 s)
+    (Hi'' : i' < S (projT1 s))
     (fi'' : bool)
     (oitem : option (vtransition_item X))
     (item := {| l := l; input := iom; destination := s; output := oom |}),
     equivocator_vlsm_transition_item_project item (Existing i' fi') = Some (oitem, Existing i' fi'').
 Proof.
   unfold vvalid in Hv. unfold vtransition in Ht.
-  simpl in Hv. simpl in Ht. simpl.
-  destruct l as (lx, descriptor). simpl in *.
+  simpl in Hv. unfold_transition Ht. unfold equivocator_vlsm_transition_item_project.
+  destruct l as (lx, descriptor). simpl in Hv. unfold snd in Ht.
   destruct s as (ns, bs).
   destruct s' as (n', bs').
   destruct descriptor as [sn | j is_equiv].
-  - destruct (vtransition X lx (sn, iom)) as (sn', om') eqn:Htx.
-    simpl in Ht. inversion Ht. subst. simpl in Hi'.
-    assert (Hi'' : i' < S n') by lia.
+  - simpl in Ht. destruct (vtransition X lx (sn, iom)) as (sn', om') eqn:Htx.
+    inversion Ht. subst. clear Ht. simpl in Hi'.
+    assert (Hi'' : i' < S (S n')) by lia.
     exists Hi''.
-    destruct (le_lt_dec (S n') i'). { lia. }
+    destruct (le_lt_dec (S (S n')) i'). { lia. }
     replace (of_nat_lt l) with (of_nat_lt Hi'') in *; try apply of_nat_ext. clear l.
     rewrite eq_dec_if_false.
     + exists false. exists None. reflexivity.
     + lia.
-  - destruct Hv as [Hj Hv]. simpl in *.
-    destruct (le_lt_dec n' j). { lia. }
+  - destruct Hv as [Hj Hv]. unfold projT1 in Ht. simpl in Hj.
+    destruct (le_lt_dec (S n') j). { lia. }
     replace (of_nat_lt l) with (of_nat_lt Hj) in *; try apply of_nat_ext. clear l.
+    simpl in Ht.
     destruct (vtransition X lx (bs' (of_nat_lt Hj), iom))
       as (si', om') eqn:Htx.
-    assert (Hi'' : i' < S n') by lia.
+    simpl in Hi'.
+    assert (Hi'' : i' < S (S n')) by lia.
     destruct is_equiv as [|] eqn:Hflag
     ; inversion Ht; subst ns om'; clear Ht
     ; apply inj_pairT2 in H1; subst bs.
-    + destruct (le_lt_dec (S n') i'). { lia. }
-      destruct (nat_eq_dec (S i') (S n')). { lia. }
+    + destruct (le_lt_dec (S (S n')) i'). { lia. }
+      destruct (nat_eq_dec (S i') (S (S n'))). { lia. }
       exists Hi''. exists false.
       exists None. reflexivity.
-    + destruct (le_lt_dec n' i'). { lia. }
+    + destruct (le_lt_dec (S n') i'). { lia. }
       destruct (nat_eq_dec j i').
       * subst j.
         rewrite eq_dec_if_true; try apply of_nat_ext.
@@ -841,36 +840,41 @@ Lemma equivocator_protocol_transition_item_project_inv5
   (fi : bool)
   : exists
     (i : nat)
-    (Hi : i < projT1 s)
+    (Hi : i < S (projT1 s))
     (d' : MachineDescriptor)
     (itemx : vtransition_item X)
     (item := {| l := l; input := iom; destination := s; output := oom |}),
     equivocator_vlsm_transition_item_project item (Existing i fi) = Some (Some itemx, d').
 Proof.
+  unfold equivocator_vlsm_transition_item_project.
   destruct s as (ns, bs).
   destruct s' as (ns', bs').
-  unfold vtransition in Ht. simpl in Ht.
+  unfold vtransition in Ht. unfold_transition Ht.
   unfold vvalid in Hv. simpl in Hv.
-  destruct l as (lx, [sn | i is_equiv]); simpl in *.
-  - destruct (vtransition X lx (sn, iom)) as (sn', om').
+  destruct l as (lx, d). unfold snd in Ht. simpl in Hv.
+  destruct d as [sn | i is_equiv].
+  - simpl in Ht.
+    destruct (vtransition X lx (sn, iom)) as (sn', om').
     inversion Ht. subst; clear Ht.
     apply inj_pairT2 in H1. subst.
-    exists ns'.  split. { lia. } exists (NewMachine sn).
-    destruct (le_lt_dec (S ns') ns'). { lia. }
+    exists (S ns').  split. { simpl; lia. } exists (NewMachine sn).
+    destruct (le_lt_dec (S (S ns')) (S ns')). { lia. }
     rewrite eq_dec_if_true; try reflexivity.
     eexists _; reflexivity.
   - destruct Hv as [Hi Hv].
-    destruct (le_lt_dec ns' i). { lia. }
+    unfold projT1 in Ht.
+    destruct (le_lt_dec (S ns') i). { lia. }
     replace (of_nat_lt l) with (of_nat_lt Hi) in *; try apply of_nat_ext. clear l.
+    simpl in Ht.
     destruct (vtransition X lx (bs' (of_nat_lt Hi), iom)) as (sn', om').
     destruct is_equiv as [|]; inversion Ht; subst; clear Ht; apply inj_pairT2 in H1; subst.
-    + exists ns'. split. { lia. }
+    + exists (S ns'). split. { simpl; lia. }
       exists (Existing i true).
-      destruct (le_lt_dec (S ns') ns'). { lia. }
+      destruct (le_lt_dec (S (S ns')) (S ns')). { lia. }
       rewrite eq_dec_if_true; try reflexivity.
       eexists _; reflexivity.
     + exists i. exists Hi. exists (Existing i false).
-      destruct (le_lt_dec ns i). { lia. }
+      destruct (le_lt_dec (S ns) i). { lia. }
       rewrite eq_dec_if_true; try reflexivity.
       eexists _; reflexivity.
 Qed.
@@ -878,26 +882,32 @@ Qed.
 Lemma preloaded_equivocator_state_project_protocol_state
   (bs : vstate equivocator_vlsm)
   (Hbs : protocol_state_prop (pre_loaded_vlsm equivocator_vlsm) bs)
-  (i : Fin.t (projT1 bs))
+  (i : Fin.t (S (projT1 bs)))
   :
   protocol_state_prop (pre_loaded_vlsm X) (projT2 bs i).
 Proof.
   revert i.
-  pose (fun bs : vstate equivocator_vlsm => forall i : t (projT1 bs), protocol_state_prop (pre_loaded_vlsm X) (projT2 bs i)) as P.
+  pose (fun bs : vstate equivocator_vlsm => forall i : t (S (projT1 bs)), protocol_state_prop (pre_loaded_vlsm X) (projT2 bs i)) as P.
   revert Hbs. revert bs.
   apply (protocol_state_prop_ind (pre_loaded_vlsm equivocator_vlsm) P)
   ; try assumption; unfold P in *; clear P; intros.
-  - destruct s as ([| [|n]], s); try inversion Hs. simpl in *. inversion i.
+  - destruct Hs as [Hzero His].
+    destruct s. simpl in *. subst x. exists None.
+    dependent destruction i; try inversion i.
+    replace (v F1) with (proj1_sig (exist _ _ His)) by reflexivity.
+     apply (protocol_initial_state (pre_loaded_vlsm X)).
   - destruct Ht as [[Hps [_ Hv]] Ht].
+    simpl in Ht. unfold vtransition in Ht. unfold_transition Ht.
     destruct l as (l, description).
-    simpl in Ht. unfold vtransition in Ht. simpl in Ht.
+    unfold snd in Ht.
     destruct description as [sn| j is_equiv].
     + destruct Hv as [Hsn Hv].
+      simpl in Ht.
       destruct (vtransition X l (sn, om)) as (sn', snom') eqn:Htx.
       inversion Ht. subst . clear Ht.
       destruct s as (ns, bs).
       simpl in *. destruct (to_nat i) as (ni, Hni).
-      destruct (nat_eq_dec ni ns); try apply Hs.
+      destruct (nat_eq_dec ni (S ns)); try apply Hs.
       subst. exists om'.
       replace (@pair (@state message (@type message (@pre_loaded_vlsm message X))) (option message) sn' om')
         with (vtransition X l (sn, om)).
@@ -909,8 +919,8 @@ Proof.
         (protocol_generated (pre_loaded_vlsm X) l sn None Hpsn
         (proj1_sig (vs0 X)) om (pre_loaded_message_protocol_prop X om) Hv).
     + destruct Hv as [Hj Hv].
-      destruct (le_lt_dec (projT1 s) j). { lia. }
-      replace (of_nat_lt l0) with (of_nat_lt Hj) in *; try apply of_nat_ext.
+      destruct (le_lt_dec (S (projT1 s)) j). { lia. }
+      replace (of_nat_lt l0) with (of_nat_lt Hj) in *; try apply of_nat_ext. clear l0.
       destruct (Hs (of_nat_lt Hj)) as [_omj Hsj].
       specialize (protocol_generated (pre_loaded_vlsm X) l (projT2 s (of_nat_lt Hj)) _omj Hsj)
         as Hgen.
@@ -918,11 +928,12 @@ Proof.
       replace (transition l (projT2 s (of_nat_lt Hj), om))
         with (vtransition X l (projT2 s (of_nat_lt Hj), om))
         in Hgen by reflexivity.
+      simpl in *.
       destruct (vtransition X l (projT2 s (of_nat_lt Hj), om)) as (sj', omj').
       destruct is_equiv as [|]; inversion Ht; subst; clear Ht; simpl in *.
       * destruct s as (ns, bs). simpl in *.
         destruct (to_nat i) as (ni, Hni).
-        destruct (nat_eq_dec ni ns); try (exists om'; assumption).
+        destruct (nat_eq_dec ni (S ns)); try (exists om'; assumption).
         apply Hs.
       * destruct (Fin.eq_dec (Fin2Restrict.n2f Hj) i); try apply Hs.
         exists om'. assumption.
@@ -933,7 +944,7 @@ Lemma equivocator_vlsm_trace_project_protocol
   (btr : list (vtransition_item equivocator_vlsm))
   (Hbtr : finite_protocol_trace_from equivocator_vlsm bs btr)
   (j : nat)
-  (Hj : j < projT1 (last (map destination btr) bs))
+  (Hj : j < S (projT1 (last (map destination btr) bs)))
   (jf : bool)
   : exists
     (tr : list (vtransition_item X))
@@ -946,7 +957,7 @@ Lemma equivocator_vlsm_trace_project_protocol
       /\ finite_protocol_trace_from X sn tr
     | Existing i fi =>
       exists
-      (Hi : i < projT1 bs)
+      (Hi : i < S (projT1 bs))
       (s := projT2 bs (of_nat_lt Hi))
       (Hlast : projT2 (last (map destination btr) bs) (of_nat_lt Hj) = last (map destination tr) s)
       ,
@@ -1014,7 +1025,7 @@ Lemma preloaded_equivocator_vlsm_trace_project_protocol
   (btr : list (vtransition_item equivocator_vlsm))
   (Hbtr : finite_protocol_trace_from (pre_loaded_vlsm equivocator_vlsm) bs btr)
   (j : nat)
-  (Hj : j < projT1 (last (map destination btr) bs))
+  (Hj : j < S (projT1 (last (map destination btr) bs)))
   (jf : bool)
   : exists
     (tr : list (vtransition_item X))
@@ -1027,7 +1038,7 @@ Lemma preloaded_equivocator_vlsm_trace_project_protocol
       /\ finite_protocol_trace_from (pre_loaded_vlsm X) sn tr
     | Existing i fi =>
       exists
-      (Hi : i < projT1 bs)
+      (Hi : i < S (projT1 bs))
       (s := projT2 bs (of_nat_lt Hi))
       (Hlast : projT2 (last (map destination btr) bs) (of_nat_lt Hj) = last (map destination tr) s)
       ,
@@ -1114,7 +1125,7 @@ Lemma preloaded_equivocator_vlsm_trace_project_protocol_inv
   (btr : list (vtransition_item equivocator_vlsm))
   (Hbtr : finite_protocol_trace_from (pre_loaded_vlsm equivocator_vlsm) bs btr)
   (i : nat)
-  (Hi : i < projT1 bs)
+  (Hi : i < S (projT1 bs))
   (fi : bool)
   : exists
     (fii : bool)
@@ -1249,25 +1260,44 @@ Lemma preloaded_equivocator_vlsm_project_protocol_trace
   (btr : list (vtransition_item equivocator_vlsm))
   (Hbtr : finite_protocol_trace (pre_loaded_vlsm equivocator_vlsm) bs btr)
   (j : nat)
-  (Hj : j < projT1 (last (map destination btr) bs))
+  (Hj : j < S (projT1 (last (map destination btr) bs)))
   (jf : bool)
   : exists
     (tr : list (vtransition_item X))
-    (sn : vstate X)
-    (Htr : equivocator_vlsm_trace_project btr (Existing j jf) = Some (tr, NewMachine sn))
-    (Hlast : projT2 (last (map destination btr) bs) (of_nat_lt Hj) = last (map destination tr) sn),
-    finite_protocol_trace (pre_loaded_vlsm X) sn tr.
+    (di : MachineDescriptor)
+    (Htr : equivocator_vlsm_trace_project btr (Existing j jf) = Some (tr, di)),
+    match di with
+    | NewMachine sn =>
+      exists
+      (Hlast : projT2 (last (map destination btr) bs) (of_nat_lt Hj) = last (map destination tr) sn),
+      finite_protocol_trace (pre_loaded_vlsm X) sn tr
+    | Existing i fi =>
+      exists
+      (Hi : i < S (projT1 bs))
+      (s := projT2 bs (of_nat_lt Hi))
+      (Hlast : projT2 (last (map destination btr) bs) (of_nat_lt Hj) = last (map destination tr) s)
+      ,
+      finite_protocol_trace (pre_loaded_vlsm X) s tr
+    end.
 Proof.
   destruct Hbtr as [Hbtr Hinit].
   destruct (preloaded_equivocator_vlsm_trace_project_protocol bs btr Hbtr j Hj jf)
     as [tr [di [Hproject Hdi]]].
   exists tr.
+  exists di.
+  exists Hproject.
   destruct di as [sn | i fi].
-  - exists sn. exists Hproject. destruct Hdi as [Hsn [Hlst Htr]].
+  - destruct Hdi as [Hsn [Hlst Htr]].
     repeat split; assumption.
   - destruct Hdi as [Hi [Hlast Htr]].
-    exfalso. apply equivocator_initial_state_empty with bs; try assumption.
-    exact (of_nat_lt Hi).
+    exists Hi. exists Hlast. split; try assumption.
+    destruct Hinit as [Hzero Hinit].
+    destruct bs as [ns bs]; simpl in *. subst ns.
+    assert (Hzero : i = 0) by lia.
+    subst i.
+    replace (of_nat_lt Hi) with (@F1 0); try assumption.
+    rewrite <- (of_nat_to_nat_inv (@F1 0)).
+    apply of_nat_ext.
 Qed.
 
 Lemma equivocator_vlsm_trace_project_output_reflecting
@@ -1329,7 +1359,7 @@ Lemma equivocator_vlsm_trace_project_inv
   (fj : bool)
   (HtrX: equivocator_vlsm_trace_project tr (Existing j fj) <> None)
   (is: state)
-  : j < projT1 (last (map destination tr) is).
+  : j < S (projT1 (last (map destination tr) is)).
 Proof.
   apply exists_last in Hntr.
   destruct Hntr as [suffix [x Heq]]. subst tr.
@@ -1346,12 +1376,12 @@ Proof.
     eqn:Hx'
   ; try discriminate Hx.
   destruct _x as [itemx|]; inversion Hx; subst lx _dmiddle; clear Hx.
-  - subst. destruct x. simpl in *.
+  - subst. destruct x. unfold equivocator_vlsm_transition_item_project in Hx'.
     destruct l. destruct destination.
-    destruct (le_lt_dec x j); try discriminate Hx'.
+    destruct (le_lt_dec (S x) j); try discriminate Hx'.
     assumption.
-  - subst. simpl in Hx'. destruct x. destruct l. destruct destination.
-    destruct (le_lt_dec x j); try discriminate Hx'.
+  - subst. unfold equivocator_vlsm_transition_item_project in Hx'. destruct x. destruct l. destruct destination.
+    destruct (le_lt_dec (S x) j); try discriminate Hx'.
     assumption.
 Qed.
 
@@ -1365,7 +1395,7 @@ Lemma preloaded_equivocator_vlsm_trace_project_protocol_inv2
   (di : MachineDescriptor)
   (trX: list (vtransition_item X))
   (HtrX: equivocator_vlsm_trace_project tr (Existing j fj) = Some (trX, di))
-  : exists (Hj : j < projT1 (last (map destination tr) is)),
+  : exists (Hj : j < S (projT1 (last (map destination tr) is))),
     match di with
     | NewMachine sn =>
       exists
@@ -1374,7 +1404,7 @@ Lemma preloaded_equivocator_vlsm_trace_project_protocol_inv2
       finite_protocol_trace_from (pre_loaded_vlsm X) sn trX
     | Existing i fi =>
       exists
-      (Hi : i < projT1 is)
+      (Hi : i < S (projT1 is))
       (Hlst : projT2 (last (map destination tr) is) (of_nat_lt Hj) = last (map destination trX) (projT2 is (of_nat_lt Hi))),
       finite_protocol_trace_from (pre_loaded_vlsm X) (projT2 is (of_nat_lt Hi)) trX
     end.
@@ -1406,11 +1436,20 @@ Lemma preloaded_equivocator_vlsm_protocol_trace_project_inv2
   (trX: list (vtransition_item X))
   (HtrX: equivocator_vlsm_trace_project tr (Existing j fj) = Some (trX, di))
   : exists
-    (Hj : j < projT1 (last (map destination tr) is))
-    (sn : vstate X)
-    (Hdi : di = NewMachine sn)
-    (Hlst : projT2 (last (map destination tr) is) (of_nat_lt Hj) = last (map destination trX) sn),
-    finite_protocol_trace (pre_loaded_vlsm X) sn trX.
+    (Hj : j < S (projT1 (last (map destination tr) is))),
+    match di with
+    | NewMachine sn =>
+      exists
+      (Hlast : projT2 (last (map destination tr) is) (of_nat_lt Hj) = last (map destination trX) sn),
+      finite_protocol_trace (pre_loaded_vlsm X) sn trX
+    | Existing i fi =>
+      exists
+      (Hi : i < S (projT1 is))
+      (s := projT2 is (of_nat_lt Hi))
+      (Hlast : projT2 (last (map destination tr) is) (of_nat_lt Hj) = last (map destination trX) s)
+      ,
+      finite_protocol_trace (pre_loaded_vlsm X) s trX
+    end.
 Proof.
   specialize (equivocator_vlsm_trace_project_inv _ Hntr j fj) as Hj.
   spec Hj. { rewrite HtrX. intro contra. discriminate contra. }
@@ -1418,9 +1457,10 @@ Proof.
   exists Hj.
   destruct
     (preloaded_equivocator_vlsm_project_protocol_trace _ _ Htr _ Hj fj)
-    as [trX' [sn [HtrX' [Hlst Hptr]]]].
+    as [trX' [di' [HtrX' Hdi]]].
   rewrite HtrX in HtrX'.
-  inversion HtrX'. subst. exists sn. exists eq_refl. exists Hlst. assumption.
+  inversion HtrX'. subst di' trX'.  clear HtrX'.
+  assumption.
 Qed.
 
 Fixpoint fin_t_listing
@@ -1458,71 +1498,83 @@ Qed.
 Section trace_mixer.
 
 Definition preloaded_protocol_equivocator_vlsm_trace_oproject
+  (is : vstate equivocator_vlsm)
   (btr : list (vtransition_item equivocator_vlsm))
-  (nj : Fin.t (projT1 (last (map destination btr) (proj1_sig (vs0 equivocator_vlsm)))))
+  (nj : Fin.t (S (projT1 (last (map destination btr) is))))
   : option (vstate X * list (vtransition_item X))
   :=
   let (j, _) := to_nat nj in
   match equivocator_vlsm_trace_project btr (Existing j false) with
   | Some (trx, NewMachine sn) => Some (sn, trx)
+  | Some (trx, Existing i _) =>
+    match (le_lt_dec (S (projT1 is)) i) with
+    | left _ => None
+    | right Hi => Some (projT2 is (of_nat_lt Hi), trx)
+    end
   | _ => None
   end.
 
 Definition equivocator_vlsm_projector_type
+  (is : vstate equivocator_vlsm)
   (btr : list (vtransition_item equivocator_vlsm))
   : Type
   :=
   forall
-    (nj : Fin.t (projT1 (last (map destination btr) (` (vs0 equivocator_vlsm))))),
+    (nj : Fin.t (S (projT1 (last (map destination btr) (is))))),
     option (vstate X * list (vtransition_item X)).
 
 Definition equivocator_projection_update
+  (is : vstate equivocator_vlsm)
   (btr : list (vtransition_item equivocator_vlsm))
-  (projector : equivocator_vlsm_projector_type btr)
-  (ni : Fin.t (projT1 (last (map destination btr) (proj1_sig (vs0 equivocator_vlsm)))))
+  (projector : equivocator_vlsm_projector_type is btr)
+  (ni : Fin.t (S (projT1 (last (map destination btr) is))))
   (ni_trace : option (vstate X * list (vtransition_item X)))
-  (nj : Fin.t (projT1 (last (map destination btr) (proj1_sig (vs0 equivocator_vlsm)))))
+  (nj : Fin.t (S (projT1 (last (map destination btr) is))))
   : option (vstate X * list (vtransition_item X))
   := 
   if Fin.eq_dec ni nj then ni_trace else projector nj.
 
 Definition preloaded_protocol_equivocator_vlsm_trace_oproject_update
+  (is : vstate equivocator_vlsm)
   (btr : list (vtransition_item equivocator_vlsm))
-  (ni : Fin.t (projT1 (last (map destination btr) (proj1_sig (vs0 equivocator_vlsm)))))
+  (ni : Fin.t (S (projT1 (last (map destination btr) is))))
   (isi : vstate X)
   (tri : list (vtransition_item X))
-  : equivocator_vlsm_projector_type btr
+  : equivocator_vlsm_projector_type is btr
   :=
-  equivocator_projection_update btr
-    (preloaded_protocol_equivocator_vlsm_trace_oproject btr)
+  equivocator_projection_update is btr
+    (preloaded_protocol_equivocator_vlsm_trace_oproject is btr)
     ni (Some (isi, tri)).
 
 Definition projection_traces
+  (is : vstate equivocator_vlsm)
   (btr : list (vtransition_item equivocator_vlsm))
-  (projector : equivocator_vlsm_projector_type btr)
-  (n := projT1 (last (map destination btr) (proj1_sig (vs0 equivocator_vlsm))))
+  (projector : equivocator_vlsm_projector_type is btr)
+  (n := projT1 (last (map destination btr) is))
   : list (vstate X * list (vtransition_item X))
   :=
-  map_option projector (fin_t_listing n).
+  map_option projector (fin_t_listing (S n)).
 
 Definition projection_traces_replace_one
+  (is : vstate equivocator_vlsm)
   (btr : list (vtransition_item equivocator_vlsm))
-  (ni : Fin.t (projT1 (last (map destination btr) (proj1_sig (vs0 equivocator_vlsm)))))
+  (ni : Fin.t (S (projT1 (last (map destination btr) is))))
   (isi : vstate X)
   (tri : list (vtransition_item X))
   : list (vstate X * list (vtransition_item X))
   :=
-  projection_traces btr
-    (preloaded_protocol_equivocator_vlsm_trace_oproject_update btr ni isi tri).
+  projection_traces is btr
+    (preloaded_protocol_equivocator_vlsm_trace_oproject_update is btr ni isi tri).
 
 Lemma projection_traces_replace_one_length
+  (is : vstate equivocator_vlsm)
   (btr : list (vtransition_item equivocator_vlsm))
-  (Hbtr : finite_protocol_trace (pre_loaded_vlsm equivocator_vlsm) (proj1_sig (vs0 equivocator_vlsm)) btr)
-  (n := projT1 (last (map destination btr) (proj1_sig (vs0 equivocator_vlsm))))
-  (ni : Fin.t n)
+  (Hbtr : finite_protocol_trace (pre_loaded_vlsm equivocator_vlsm) is btr)
+  (n := projT1 (last (map destination btr) is))
+  (ni : Fin.t (S n))
   (isi : vstate X)
   (tri : list (vtransition_item X))
-  : length (projection_traces_replace_one btr ni isi tri) = n.
+  : length (projection_traces_replace_one is btr ni isi tri) = S n.
 Proof.
   unfold projection_traces_replace_one.
   unfold projection_traces.
@@ -1539,17 +1591,20 @@ Proof.
     destruct (to_nat nj) as [j Hj] eqn:Heqnj.
     destruct
       (preloaded_equivocator_vlsm_project_protocol_trace _ _ Hbtr _ Hj false)
-      as [trX [snX [Hproject _]]].
+      as [trX [di [Hproject Hdi]]].
     rewrite Hproject.
-    intro contra. discriminate contra.
+    destruct di as [sn | i fi].
+    + intro contra. discriminate contra.
+    + destruct Hdi as [Hi [HlstX [HtrX]]].
+      destruct (le_lt_dec (S (projT1 is)) i). { lia. }
+      intro contra. discriminate contra.
 Qed.
 
 Context
   (goal_state : vstate equivocator_vlsm)
   (n := projT1 goal_state)
-  (Hnz : 0 < n)
   (traces : list (vstate X * list (vtransition_item X)))
-  (Hn : length traces = n)
+  (Hn : length traces = S n)
   (Htraces : Forall
     (fun trace => 
       finite_protocol_trace (pre_loaded_vlsm X) (fst trace) (snd trace)
@@ -1557,7 +1612,7 @@ Context
     traces)
   (Hne_traces : Forall (fun trace => snd trace <> []) traces)
   (Hs
-    : forall i : Fin.t n,
+    : forall i : Fin.t (S n),
       let (ni, _) := to_nat i in
       match nth ni traces (proj1_sig (vs0 X), []) with (isi, tri) =>
         last (map destination tri) isi = projT2 goal_state i
@@ -1579,7 +1634,7 @@ Definition lift_trace_to_equivocator
     :: fold_right
       (fun lab tr =>
         match lab with {| l := lx; input := iom; output := oom; destination := sx |} =>
-          {| l := mk_label lx  (Existing i false); input := iom; output := oom; destination := equivocator_state_extend start sx |}
+          {| l := mk_label lx  (Existing (S i) false); input := iom; output := oom; destination := equivocator_state_extend start sx |}
           :: tr
         end)
       [] tri
@@ -1629,7 +1684,7 @@ Definition equivocator_has_been_sent
   let (n, bs) := s in
   existsb
     (fun i => has_been_sent X (bs i) m)
-    (fin_t_listing n).
+    (fin_t_listing (S n)).
 
 Lemma equivocator_has_been_sent_consistency
   (s : vstate equivocator_vlsm)
@@ -1650,8 +1705,7 @@ Proof.
     specialize
       (preloaded_equivocator_vlsm_protocol_trace_project_inv2 _ _ Hntr Hbtr _ _ _ _ Hproject)
       as HpreX.
-    rewrite Hlast in HpreX. destruct HpreX as [Hj [sn [Hi [Hlastx HtrX]]]].
-    symmetry in Hlastx. subst i.
+    rewrite Hlast in HpreX. destruct HpreX as [Hj Hi].
     assert (Hsj : protocol_state_prop (pre_loaded_vlsm X) (projT2 s (Fin2Restrict.n2f Hj))).
     { simpl.  simpl in *.
       specialize
@@ -1663,18 +1717,30 @@ Proof.
     }
     assert (Hall : selected_message_exists_in_all_traces X output (projT2 s (of_nat_lt Hj)) m).
     { apply has_been_sent_consistency; try assumption.
-      exists sn. exists trX. exists HtrX. exists Hlastx. assumption. 
+      destruct i as [sn | i fi].
+      - destruct Hi as [Hlastx HtrX].
+        symmetry in Hlastx.
+        exists sn. exists trX. exists HtrX. exists Hlastx. assumption.
+      - destruct Hi as [Hi [Hlastx HtrX]].
+        exists (projT2 bis (of_nat_lt Hi)). exists trX. exists HtrX.
+        symmetry in Hlastx. exists Hlastx.
+        assumption.
     }
     clear -Hall.
     intros bis btr Hbtr Hlast.
     subst s.
     destruct
       (preloaded_equivocator_vlsm_project_protocol_trace _ _ Hbtr _ Hj false)
-      as [trX [sn [Hproject [Hlast HtrX]]]].
+      as [trX [di [Hproject Hdi]]].
     apply
       (equivocator_vlsm_trace_project_output_reflecting _ _ _ _ Hproject m).
-    symmetry in Hlast.
-    apply (Hall _ _ HtrX Hlast).
+    destruct di as [sn | i fi].
+    + destruct Hdi as [Hlast HtrX].
+      symmetry in Hlast.
+      apply (Hall _ _ HtrX Hlast).
+    + destruct Hdi as [Hi [Hlast HtrX]].
+      symmetry in Hlast.
+      apply (Hall _ _ HtrX Hlast).
   - intro Hall.
     destruct Hs as [om Hs].
     apply (protocol_is_trace (pre_loaded_vlsm equivocator_vlsm)) in Hs.
@@ -1710,31 +1776,32 @@ Proof.
          (@state message (@type message equivocator_vlsm))
          (@destination message
             (@type message equivocator_vlsm)) tr) start)
-      with (existT (fun n : nat => t n -> vstate X) n bs)
+      with (existT (fun n : nat => t (S n) -> vstate X) n bs)
       in Hpre.
     simpl in Hpre.
     destruct (to_nat j) as [nj Hnj].  simpl in *.
     specialize (Hpre nj Hnj false).
-    destruct Hpre as [trX [sn [Hproject [HlastX HtrX]]]].
-    symmetry in HlastX.
-    rewrite Hj in HlastX.
-    spec Hjbs sn trX HtrX HlastX.
-    apply equivocator_vlsm_trace_project_output_reflecting with trX (Existing nj false) (NewMachine sn)
-    ; assumption.
+    destruct Hpre as [trX [di [Hproject Hdi]]].
+    destruct di as [sn | i fi].
+    + destruct Hdi as [HlastX HtrX].
+      symmetry in HlastX.
+      rewrite Hj in HlastX.
+      spec Hjbs sn trX HtrX HlastX.
+      apply equivocator_vlsm_trace_project_output_reflecting with trX (Existing nj false) (NewMachine sn)
+      ; assumption.
+    + destruct Hdi as [Hi [HlastX HtrX]].
+      symmetry in HlastX.
+      rewrite Hj in HlastX.
+      spec Hjbs (projT2 start (of_nat_lt Hi)) trX HtrX HlastX.
+      apply equivocator_vlsm_trace_project_output_reflecting with trX (Existing nj false) (Existing i fi)
+      ; assumption.
   - intro Hbbs. assert (Hbbs' := Hbbs).
     destruct Hs as [om Hs].
     apply (protocol_is_trace (pre_loaded_vlsm equivocator_vlsm)) in Hs.
     destruct Hs as [Hinit | [is [tr [Htr [Hlast _]]]]]
     ; try (elim (selected_message_exists_in_all_traces_initial_state equivocator_vlsm s Hinit output m)
       ; assumption).
-    assert (Hsnz : projT1 s <> 0).
-    { intro contra.
-      assert (Hinit : vinitial_state_prop (equivocator_vlsm) s) by assumption.
-      elim (selected_message_exists_in_all_traces_initial_state equivocator_vlsm s Hinit output m).
-      assumption.
-    }
-    assert (Hsz : 0 < projT1 s) by lia.
-    specialize (lift_traces_to_equivocator_protocol_trace s Hsz) as Hlift_protocol_trace.
+    specialize (lift_traces_to_equivocator_protocol_trace s) as Hlift_protocol_trace.
     assert (Hlst := last_error_destination_last _ _ Hlast is).
     spec Hbbs is tr Htr Hlst.
     destruct
@@ -1749,7 +1816,8 @@ Proof.
     specialize
       (preloaded_equivocator_vlsm_protocol_trace_project_inv2 _ _ Hntr Htr _ _ _ _ HtrX)
       as HpreX.
-    rewrite Hlst in HpreX. simpl in HpreX. destruct HpreX as [Hj [sn [Hi [Hlstx Htrx]]]].
+    rewrite Hlst in HpreX. simpl in HpreX.
+    destruct HpreX as [Hj Hi].
     unfold equivocator_has_been_sent.
     destruct s as (ns, bs). simpl in Hlift_protocol_trace.
     apply existsb_exists.
@@ -1765,8 +1833,15 @@ Proof.
     }
     apply (proper_sent X); try assumption.
     apply has_been_sent_consistency; try assumption.
-    exists sn. exists trX. exists Htrx. symmetry in Hlstx. exists Hlstx.
-    assumption.
+    destruct i as [sn | i fi].
+    + destruct Hi as [Hlstx Htrx].
+      exists sn. exists trX. exists Htrx. symmetry in Hlstx. exists Hlstx.
+      assumption.
+    + destruct Hi as [Hi [Hlstx Htrx]].
+      exists (projT2 is (of_nat_lt Hi)).
+      exists trX. exists Htrx.
+      symmetry in Hlstx. exists Hlstx.
+      assumption.
 Qed.
 
 Lemma equivocator_proper_not_sent
@@ -1806,7 +1881,7 @@ Definition equivocator_sent_messages_fn
   : set message
   :=
   fold_right (set_union eq_dec) []
-    (map (fun i => sent_messages_fn X (projT2 s i)) (fin_t_listing (projT1 s))).
+    (map (fun i => sent_messages_fn X (projT2 s i)) (fin_t_listing (S (projT1 s)))).
 
 Lemma equivocator_sent_messages_full
   (s : vstate equivocator_vlsm)
@@ -1827,10 +1902,14 @@ Proof.
     destruct Hs as [om Hs].
     apply (protocol_is_trace (pre_loaded_vlsm equivocator_vlsm)) in Hs.
     destruct Hs as [Hs | [is [tr [Htr [Hlast _]]]]].
-    + specialize (Hm (projT2 s i) []). spec Hm.
+    + specialize (Hm (projT2 s i) []).
+      spec Hm.
       { split.
         - apply (finite_ptrace_empty (pre_loaded_vlsm X)). assumption.
-        - exfalso. apply equivocator_initial_state_empty with s; assumption.
+        - destruct Hs as [Hzero His].
+          destruct s as [n s]. simpl in *. subst n.
+          dependent destruction i; try inversion i.
+          assumption.
       }
       specialize (Hm eq_refl). inversion Hm.
     + specialize (last_error_destination_last _ _ Hlast is) as Hlst. clear Hlast.
@@ -1842,11 +1921,18 @@ Proof.
       subst s.
       destruct
         (preloaded_equivocator_vlsm_project_protocol_trace _ _ Htr _ Hi false)
-        as [trX [sn [Hzero [Hlast HtrX]]]].
-      apply equivocator_vlsm_trace_project_output_reflecting with trX (Existing ni false) (NewMachine sn)
-      ; try assumption.
-      symmetry in Hlast.
-      apply (Hm _ _ HtrX Hlast).
+        as [trX [di Hdi]].
+      destruct di as [sn | i fi].
+      * destruct Hdi as [Hproject [Hlast HtrX]].
+        apply equivocator_vlsm_trace_project_output_reflecting with trX (Existing ni false) (NewMachine sn)
+        ; try assumption.
+        symmetry in Hlast.
+        apply (Hm _ _ HtrX Hlast).
+      * destruct Hdi as [Hproject [Hi' [Hlast HtrX]]].
+        apply equivocator_vlsm_trace_project_output_reflecting with trX (Existing ni false) (Existing i fi)
+        ; try assumption.
+        symmetry in Hlast.
+        apply (Hm _ _ HtrX Hlast).
   - intros [[m' Hm] Heq]. simpl in Heq. subst m'.
     destruct Hm as [is [tr [Htr [Hlst Hexists]]]].
     destruct
@@ -1862,7 +1948,7 @@ Proof.
       (preloaded_equivocator_vlsm_protocol_trace_project_inv2 _ _ Hntr Htr _ _ _ _ Hproject)
       as HpreX.
     rewrite Hlst in HpreX.
-    destruct HpreX as [Hi [sstart [Histart [Hlast HtrX]]]].
+    destruct HpreX as [Hi Histart].
     apply set_union_in_iterated. apply Exists_exists.
     exists (sent_messages_fn X (projT2 s (of_nat_lt Hi))).
     split.
@@ -1871,7 +1957,14 @@ Proof.
     + apply (sent_messages_full X); try apply HpsX.
       assert (Hm : selected_message_exists_in_some_traces X output (projT2 s (of_nat_lt Hi)) m)
       ; try (exists (exist _ m Hm); reflexivity).
-      * exists sstart. exists trX. exists HtrX. symmetry in Hlast. exists Hlast.
+      destruct istart as [sstart | istart fstart].
+      * destruct Histart as [Hlast HtrX].
+        exists sstart. exists trX. exists HtrX. symmetry in Hlast. exists Hlast.
+        assumption.
+      * destruct Histart as [Histart [Hlast HtrX]].
+        exists (projT2 is (of_nat_lt Histart)).
+        exists trX. exists HtrX.
+        symmetry in Hlast. exists Hlast.
         assumption.
 Qed.
 
@@ -1968,28 +2061,56 @@ Definition equivocators_no_equivocations_vlsm
   :=
   composite_vlsm equivocator_IM (partition i0) equivocators_no_equivocations_constraint.
 
-Definition equivocators_state_project
+Definition equivocators_state_project'
   (s : vstate equivocators_no_equivocations_vlsm)
-  (Hzero : forall e : equiv_index, 0 < projT1 (s (inl e)))
   (pi : equiv_index + nequiv_index)
   : vstate (IM (rpartition pi))
   :=
   match pi with
-  | inl e => projT2 (s (inl e)) (of_nat_lt (Hzero e))
+  | inl e => projT2 (s (inl e)) (of_nat_lt (Hzero _ (s (inl e))))
   | inr n => s (inr n)
   end.
+
+Definition equivocators_state_project
+  (s : vstate equivocators_no_equivocations_vlsm)
+  (i : index)
+  : vstate (IM i).
+Proof.
+  pose (equivocators_state_project' s (partition i)) as si.
+  rewrite Hlpartition in si.
+  exact si.
+Defined.
+
+Definition equivocators_label_project
+  (l : vlabel equivocators_no_equivocations_vlsm)
+  : option (vlabel X)
+:=
+let (i, li) := l in
+match i as s return (vlabel (equivocator_IM s) -> option (vlabel X)) with
+| inl e =>
+	fun li0 : vlabel (equivocator_IM (inl e)) =>
+    let (lj, dj) := li0 in
+    match dj with
+    | Existing _ 0 false =>
+      Some (existT (fun n : index => vlabel (IM n)) (rpartition (inl e)) lj)
+    | _ => None
+    end
+| inr n =>
+    fun li0 : vlabel (equivocator_IM (inr n)) =>
+    Some (existT (fun n0 : index => vlabel (IM n0)) (rpartition (inr n)) li0)
+end li.
 
 Definition equivocators_transition_item_project
   (item : vtransition_item equivocators_no_equivocations_vlsm)
   : option (vtransition_item X)
   :=
   match item with {| l := el; input := iom; output := oom; destination := s |} =>
-    let (i, li) := el in
-    match i with
-    | inl _ => None
-    | inr _ => None
+    match  equivocators_label_project el with
+    | None => None
+    | Some lx =>
+      let sx := equivocators_state_project s in
+      Some {| l := lx; input := iom; output := oom; destination := sx |}
     end
   end.
-
 
 End fully_equivocating_composition.
